Add a proper semantics for REP MOVSB
This sets up a function "x86_movsb" implementing the explicitly
sequential byte copy specified in the ISA. We also introduce
and justify the function "x86_stringcopy" which factors the
operation into an update involving the input and output buffers
only, which is more useful in actual simulations.

x86/proofs/instruction.ml
@@ -267,7 +267,7 @@ let instruction_INDUCTION,instruction_RECURSION = define_type
    | MOV operand operand
    | MOVD operand operand
    | MOVQ operand operand
-   | MOVSB operand operand operand
+   | MOVSB bool operand operand operand
    | MOVSX operand operand
    | MOVZX operand operand
    | MOVAPS operand operand
